

Q(4)

Repeat until $J(\theta)$ stops improving:

$$\theta_j \leftarrow \theta_j - \alpha \frac{1}{2} \sum_{i=1}^m (X^{(i)}_j - Y^{(i)})$$

$$\theta_j \leftarrow \theta_j - \alpha \frac{\partial J(\theta)}{\partial \theta_j}$$

$$\text{where } J(\theta) = \frac{1}{2} \sum_{i=1}^m (X^{(i)} \theta - Y^{(i)})^2$$

$$\frac{\partial J}{\partial \theta_j} = \sum_{i=1}^m (X^{(i)} \theta - Y^{(i)}) X^{(i)}_j$$

$\rightarrow j^{\text{th}}$ feature of i^{th} training example.

$$\Rightarrow \theta_j \leftarrow \theta_j - \alpha \sum_{i=1}^m (X^{(i)} \theta - Y^{(i)}) X^{(i)}_j, j = 1, 2, \dots, n$$

Pseudo code

Repeat

{ For $j = 1, 2, \dots, n$

$$\theta_j \leftarrow \theta_j - \alpha \sum_{i=1}^m (X^{(i)} \theta - Y^{(i)}) X^{(i)}_j }$$

until $J(\theta)$ stops improving.